verification/gen/SlhVerify/TypesExternal.lean
@@ -14,10 +14,4 @@ set_option maxHeartbeats 1000000
 /- You can set the `maxRecDepth` value with the `-max-recdepth` CLI option -/
 set_option maxRecDepth 2048
 
-/-- [core::num::error::TryFromIntError]
-    Source: '/rustc/library/core/src/num/error.rs', lines 10:0-10:26
-    Name pattern: [core::num::error::TryFromIntError]
-    Visibility: public -/
-@[rust_type "core::num::error::TryFromIntError"]
-axiom core.num.error.TryFromIntError : Type
 
